Only encrypt payload

src/lib/communication/DY.Lib.Communication.Core.fst
@@ -21,22 +21,9 @@ type communication_message = {
 %splice [ps_communication_message_is_well_formed] (gen_is_well_formed_lemma (`communication_message))
 
 [@@with_bytes bytes]
-type pkenc_input =
-  | PkEncInput: payload:bytes -> pkenc_input
-  | PkEncSignInput: cm:communication_message -> pkenc_input
-
-#push-options "--ifuel 1 --fuel 0"
-%splice [ps_pkenc_input] (gen_parser (`pkenc_input))
-%splice [ps_pkenc_input_is_well_formed] (gen_is_well_formed_lemma (`pkenc_input))
-#pop-options
-
-instance parseable_serializeable_bytes_pkenc_input: parseable_serializeable bytes pkenc_input
-  = mk_parseable_serializeable ps_pkenc_input
-
-[@@with_bytes bytes]
 type signature_input = 
   | Plain: msg:communication_message -> signature_input
-  | Encrypted: pk:bytes -> payload:bytes -> signature_input
+  | Encrypted: pk:bytes -> msg:communication_message -> signature_input
 
 #push-options "--ifuel 1 --fuel 0"
 %splice [ps_signature_input] (gen_parser (`signature_input))
@@ -48,7 +35,7 @@ instance parseable_serializeable_bytes_signature_input: parseable_serializeable 
 
 [@@with_bytes bytes]
 type communication_message_sign = {
-  payload:bytes;
+  msg:bytes;
   signature:bytes;
 }
 
@@ -103,10 +90,9 @@ let comm_label sender receiver = join (principal_label sender) (principal_label 
 
 (**** Confidential Send and Receive Functions ****)
 
-val encrypt_message: bytes -> bytes -> pkenc_input -> bytes
+val encrypt_message: bytes -> bytes -> bytes -> bytes
 let encrypt_message pk_receiver nonce payload =
-  let payload_bytes = serialize pkenc_input payload in
-  pk_enc pk_receiver nonce payload_bytes
+  pk_enc pk_receiver nonce payload
 
 val send_confidential:
   communication_keys_sess_ids ->
@@ -116,15 +102,14 @@ let send_confidential comm_keys_ids sender receiver payload =
   let*? pk_receiver = get_public_key sender comm_keys_ids.pki (LongTermPkEncKey comm_layer_pkenc_tag) receiver in
   let* nonce = mk_rand PkNonce (long_term_key_label sender) 32 in
   trigger_event sender (CommConfSendMsg sender receiver payload);*
-  let msg_encrypted = encrypt_message pk_receiver nonce (PkEncInput payload) in
+  let msg_encrypted = encrypt_message pk_receiver nonce payload in
   let* msg_id = send_msg msg_encrypted in
   return (Some msg_id)
 
 
-val decrypt_message: bytes -> bytes -> option pkenc_input
+val decrypt_message: bytes -> bytes -> option bytes
 let decrypt_message sk_receiver msg_encrypted =
-  let? payload_bytes = pk_dec sk_receiver msg_encrypted in
-  parse pkenc_input payload_bytes
+  pk_dec sk_receiver msg_encrypted
 
 val receive_confidential:
   communication_keys_sess_ids ->
@@ -133,9 +118,7 @@ val receive_confidential:
 let receive_confidential comm_keys_ids receiver msg_id =
   let*? sk_receiver = get_private_key receiver comm_keys_ids.private_keys (LongTermPkEncKey comm_layer_pkenc_tag) in
   let*? msg_encrypted = recv_msg msg_id in
-  let*? pkenc_in:pkenc_input = return (decrypt_message sk_receiver msg_encrypted) in
-  return (guard (PkEncInput? pkenc_in));*?
-  let payload = PkEncInput?.payload pkenc_in in
+  let*? payload = return (decrypt_message sk_receiver msg_encrypted) in
   trigger_event receiver (CommConfReceiveMsg receiver payload);*
   return (Some payload)
 
@@ -144,18 +127,19 @@ let receive_confidential comm_keys_ids receiver msg_id =
 
 val sign_message: principal -> principal -> bytes -> bytes -> bool -> bytes -> bytes -> bytes
 let sign_message sender receiver payload pk_receiver is_encrypted sk nonce =
+  let msg:communication_message = {sender; receiver; payload} in
   if is_encrypted then (
-    let sig_input = Encrypted pk_receiver payload in
+    let sig_input = Encrypted pk_receiver msg in
     let sig_input_bytes = serialize signature_input sig_input in
     let signature = sign sk nonce sig_input_bytes in
-    let msg_signed = {payload=sig_input_bytes; signature} in
-    serialize communication_message_sign msg_signed
+    let signed_msg = {msg=sig_input_bytes; signature} in
+    serialize communication_message_sign signed_msg
   ) else (
-    let sig_input = Plain {sender; receiver; payload} in
+    let sig_input = Plain msg in
     let sig_input_bytes = serialize signature_input sig_input in
     let signature = sign sk nonce sig_input_bytes in
-    let msg_signed = {payload=sig_input_bytes; signature} in
-    serialize communication_message_sign msg_signed
+    let signed_msg = {msg=sig_input_bytes; signature} in
+    serialize communication_message_sign signed_msg
   )
 
 val send_authenticated:
@@ -171,59 +155,55 @@ let send_authenticated comm_keys_ids sender receiver payload =
   return (Some msg_id)
 
 #push-options "--ifuel 1 --fuel 0"
-val verify_message: principal -> bytes -> bool -> bytes -> option bytes
-let verify_message receiver msg_bytes is_encrypted vk_sender =
-  let? msg_signed = parse communication_message_sign msg_bytes in
-  let? sign_input = parse signature_input msg_signed.payload in
+val verify_message: principal -> bytes -> bytes -> option communication_message
+let verify_message receiver sign_msg_bytes vk_sender =
+  let? msg_sign = parse communication_message_sign sign_msg_bytes in
+  let? sign_input = parse signature_input msg_sign.msg in
+  guard (verify vk_sender msg_sign.msg msg_sign.signature);?
   match sign_input with
-  | Plain cm -> (
-    guard (verify vk_sender msg_signed.payload msg_signed.signature);?
+  | Plain cm -> (    
     guard (cm.receiver = receiver);?
-    Some cm.payload
+    Some cm
   )
-  | Encrypted pk_receiver payload -> (
-    guard (verify vk_sender msg_signed.payload msg_signed.signature);?
-    //guard (msg_signed.receiver = receiver);?
-    //guard (DY.Core.Bytes.Type.PkEnc? msg_signed.payload);?
-    Some payload
+  | Encrypted pk_receiver cm -> (
+    guard (cm.receiver = receiver);?
+    Some cm
   )
-#pop-options
 
-val parse_sig_message: bytes -> option communication_message
-let parse_sig_message msg_bytes =
-  let? msg = parse communication_message_sign msg_bytes in
-  let? sign_input = parse signature_input msg.payload in
-  guard(Plain? sign_input);?
-  Some (Plain?.msg sign_input)
+// This function is used to implicitly check that the signature input has to
+// correct type (Plain in this case)
+val get_sender: bytes -> option principal
+let get_sender msg_bytes =
+  let? msg_sign = parse communication_message_sign msg_bytes in
+  let? sign_input = parse signature_input msg_sign.msg in
+  match sign_input with
+  | Plain cm -> Some cm.sender
+  | Encrypted pk_receiver cm -> None
+#pop-options
 
 val receive_authenticated:
   communication_keys_sess_ids ->
   principal -> timestamp ->
   traceful (option communication_message)
 let receive_authenticated comm_keys_ids receiver msg_id =
-  let*? msg_signed = recv_msg msg_id in
-  let*? msg:communication_message = return (parse_sig_message msg_signed) in
-  let*? vk_sender = get_public_key receiver comm_keys_ids.pki (LongTermSigKey comm_layer_sign_tag) msg.sender in
-  let*? payload = return (verify_message receiver msg_signed false vk_sender) in
-  trigger_event receiver (CommAuthReceiveMsg msg.sender receiver msg.payload);*
-  return (Some msg)
+  let*? msg_signed_bytes = recv_msg msg_id in
+  let*? sender = return (get_sender msg_signed_bytes) in
+  let*? vk_sender = get_public_key receiver comm_keys_ids.pki (LongTermSigKey comm_layer_sign_tag) sender in
+  let*? cm = return (verify_message receiver msg_signed_bytes vk_sender) in
+  trigger_event receiver (CommAuthReceiveMsg cm.sender receiver cm.payload);*
+  return (Some cm)
 
 (**** Confidential and Authenticates Send and Receive Functions ****)
 
 val encrypt_and_sign_message: principal -> principal -> bytes -> bytes -> bytes -> bytes -> bytes -> bytes
 let encrypt_and_sign_message sender receiver payload pk_receiver sk_sender enc_nonce sign_nonce =
-  let pkenc_sign_input = PkEncSignInput {sender; receiver; payload} in
-  let enc_payload = encrypt_message pk_receiver enc_nonce pkenc_sign_input in
+  let enc_payload = encrypt_message pk_receiver enc_nonce payload in
   sign_message sender receiver enc_payload pk_receiver true sk_sender sign_nonce
 
-// TODO remove comment if proof works
-// We do not encrypt the sender and receiver
-// because, in real-world settings, they can also
-// be identified by the IP addresses or
-// certificates they use. Having the sender and
-// receiver as plaintext allows us to reuse the
-// functions to create and parse confidential and
-// authenticated messages.
+// We do not encrypt the sender and receiver because, in real-world settings,
+// they can also be identified by the IP addresses or certificates they use.
+// Having the sender and receiver as plaintext allows us to reuse the functions
+// to create and parse confidential and authenticated messages.
 val send_confidential_authenticated:
   communication_keys_sess_ids ->
   principal -> principal -> bytes ->
@@ -239,17 +219,24 @@ let send_confidential_authenticated comm_keys_ids sender receiver payload =
   let* msg_id = send_msg msg_encrypted_signed_bytes in
   return (Some msg_id)
 
-val decrypt_signed_message: principal -> bytes -> bytes -> option communication_message
-let decrypt_signed_message receiver sk_receiver msg_encrypted_signed =
-  let? signed_msg = parse communication_message_sign msg_encrypted_signed in
-  let? signature_in = parse signature_input signed_msg.payload in
-  guard(Encrypted? signature_in);?
-  guard((Encrypted?.pk signature_in) = pk sk_receiver);?
-  let? pkenc_in = decrypt_message sk_receiver (Encrypted?.payload signature_in) in 
-  guard(PkEncSignInput? pkenc_in);?
-  let cm = PkEncSignInput?.cm pkenc_in in
-  guard(cm.receiver = receiver);?
-  Some cm
+val validate_signature_input: bytes -> bool -> bytes -> option bool
+let validate_signature_input msg is_encrypted sk_receiver =
+  let? msg_sign = parse communication_message_sign msg in
+  let? sign_input = parse signature_input msg_sign.msg in
+  if not is_encrypted then
+    Some (Plain? sign_input)
+  else
+    Some (Encrypted? sign_input && (Encrypted?.pk sign_input) = pk sk_receiver)
+
+val verify_and_decrypt_message: principal -> bytes -> bytes -> bytes -> option communication_message
+let verify_and_decrypt_message receiver sk_receiver vk_sender msg_encrypted_signed =
+  let? cm = verify_message receiver msg_encrypted_signed vk_sender in
+
+  let? validation_result = validate_signature_input msg_encrypted_signed true sk_receiver in
+  guard(validation_result);?
+
+  let? payload = decrypt_message sk_receiver cm.payload in
+  Some ({cm with payload})
 
 val receive_confidential_authenticated:
   communication_keys_sess_ids ->
@@ -258,9 +245,9 @@ val receive_confidential_authenticated:
 let receive_confidential_authenticated comm_keys_ids receiver msg_id =
   let*? msg_encrypted_signed = recv_msg msg_id in
   let*? sk_receiver = get_private_key receiver comm_keys_ids.private_keys (LongTermPkEncKey comm_layer_pkenc_tag) in
-  let*? cm:communication_message = return (decrypt_signed_message receiver sk_receiver msg_encrypted_signed) in  
-  let*? vk_sender = get_public_key receiver comm_keys_ids.pki (LongTermSigKey comm_layer_sign_tag) cm.sender in
-  let*? _ = return (verify_message receiver msg_encrypted_signed true vk_sender) in  
+  let*? sender = return (get_sender msg_encrypted_signed) in
+  let*? vk_sender = get_public_key receiver comm_keys_ids.pki (LongTermSigKey comm_layer_sign_tag) sender in 
+  let*? cm:communication_message = return (verify_and_decrypt_message receiver sk_receiver vk_sender msg_encrypted_signed) in 
   trigger_event receiver (CommConfAuthReceiveMsg cm.sender receiver cm.payload);*
   return (Some cm)
 
